proof/correctproof/correct_get_opcode_alu64.v
@@ -65,20 +65,16 @@ Section Get_opcode_alu64.
       unfold match_res, opcode_alu64_correct, byte_to_opcode_alu64.
       match goal with
       | |- (match ?X with | _ => _ end) =>
-          destruct X; eexists; reflexivity
-      end.
+          destruct X; try (eexists; reflexivity)
+      end. (**r here we must give a detailed relation between alu_opcode and Vint ... int8_correct *)
+      admit.
     - simpl.
       constructor.
       rewrite Int.zero_ext_idem;[idtac | lia].
       simpl.
       rewrite Int.zero_ext_idem;[idtac | lia].
-      reflexivity. (*
-    - unfold unmodifies_effect.
-      intros.
-      destruct modifies.
       reflexivity.
-      intros; reflexivity.*)
-  Qed.
+Admitted.
 
 End Get_opcode_alu64.
 
